Rephrased example in terms of Even/Odd rather than yes/no

fairness/examples/yesno_incr/yesno_incr.v
@@ -29,36 +29,36 @@ Definition start : val :=
 
 (** * Definition of the model! *)
 
-Inductive YN := Y | No.
+Inductive EO := ρEven | ρOdd.
 
-#[global] Instance YN_eqdec: EqDecision YN.
+#[global] Instance EO_eqdec: EqDecision EO.
 Proof. solve_decision. Qed.
 
-#[global] Instance YN_countable: Countable YN.
+#[global] Instance EO_countable: Countable EO.
 Proof.
   refine ({|
-             encode yn := match yn with Y => 1 | No => 2 end;
-             decode p := match p with 1 => Some Y | 2 => Some No | _ => None end;
+             encode eo := match eo with ρEven => 1 | ρOdd => 2 end;
+             decode p := match p with 1 => Some ρEven | 2 => Some ρOdd | _ => None end;
          |})%positive.
-  intros yn. by destruct yn.
+  intros eo. by destruct eo.
 Qed.
 
-#[global] Instance YN_inhabited: Inhabited YN.
-Proof. exact (populate Y). Qed.
+#[global] Instance EO_inhabited: Inhabited EO.
+Proof. exact (populate ρEven). Qed.
 
-Inductive yntrans: nat -> option YN -> nat -> Prop :=
-| yes_trans n : Nat.even n → yntrans n (Some Y) (S n)
-| yes_fail n : Nat.odd n → yntrans n (Some Y) n
-| no_trans n : Nat.odd n → yntrans n (Some No) (S n)
-| no_fail n : Nat.even n → yntrans n (Some No) n
+Inductive eotrans: nat -> option EO -> nat -> Prop :=
+| even_trans n : Nat.even n → eotrans n (Some ρEven) (S n)
+| even_fail n : Nat.odd n → eotrans n (Some ρEven) n
+| no_trans n : Nat.odd n → eotrans n (Some ρOdd) (S n)
+| no_fail n : Nat.even n → eotrans n (Some ρOdd) n
 .
 
-Definition yn_live_roles : gset YN := {[ No; Y ]}.
+Definition eo_live_roles : gset EO := {[ ρOdd; ρEven ]}.
 
 Lemma live_spec_holds :
-  forall s ρ s', yntrans s (Some ρ) s' -> ρ ∈ yn_live_roles.
+  forall s ρ s', eotrans s (Some ρ) s' -> ρ ∈ eo_live_roles.
 Proof.
-  intros n yn n' Htrans. rewrite /yn_live_roles.
+  intros n eo n' Htrans. rewrite /eo_live_roles.
   inversion Htrans; simplify_eq; try set_solver; try lia; destruct n'; try set_solver; lia.
 Qed.
 
@@ -66,9 +66,9 @@ Definition the_fair_model: FairModel.
 Proof.
   refine({|
             fmstate := nat;
-            fmrole := YN;
-            fmtrans := yntrans;
-            live_roles _ := yn_live_roles;
+            fmrole := EO;
+            fmtrans := eotrans;
+            live_roles _ := eo_live_roles;
             fm_live_spec := live_spec_holds;
           |}).
 Defined.
@@ -79,31 +79,29 @@ Definition the_model: LiveModel heap_lang the_fair_model :=
   |}.
 
 (** The CMRAs we need. *)
-Class yesnoG Σ := YesnoG {
-  yes_name: gname;
-  no_name: gname;
-  yesno_n_G :> inG Σ (excl_authR natO);
-  yesno_f_G :> inG Σ (excl_authR boolO);
+Class evenoddG Σ := EvenoddG {
+  even_name: gname;
+  odd_name: gname;
+  evenodd_n_G :> inG Σ (excl_authR natO);
  }.
-Class yesnoPreG Σ := {
-  yesno_PreG :> inG Σ (excl_authR natO);
-  yesno_f_PreG :> inG Σ (excl_authR boolO);
+Class evenoddPreG Σ := {
+  evenodd_PreG :> inG Σ (excl_authR natO);
  }.
-Definition yesnoΣ : gFunctors :=
+Definition evenoddΣ : gFunctors :=
   #[ heapΣ the_fair_model; GFunctor (excl_authR natO) ; GFunctor (excl_authR boolO) ].
 
-Global Instance subG_yesnoΣ {Σ} : subG yesnoΣ Σ → yesnoPreG Σ.
+Global Instance subG_evenoddΣ {Σ} : subG evenoddΣ Σ → evenoddPreG Σ.
 Proof. solve_inG. Qed.
 
 Section proof.
-  Context `{!heapGS Σ the_model, !yesnoG Σ}.
-  Let Ns := nroot .@ "yes_no".
+  Context `{!heapGS Σ the_model, !evenoddG Σ}.
+  Let Ns := nroot .@ "even_odd".
 
-  Definition yes_at (n: nat) := own yes_name (◯E n).
-  Definition no_at (n: nat) := own no_name (◯E n).
+  Definition even_at (n: nat) := own even_name (◯E n).
+  Definition odd_at (n: nat) := own odd_name (◯E n).
 
-  Definition auth_yes_at (n: nat) := own yes_name (●E n).
-  Definition auth_no_at (n: nat) := own no_name (●E n).
+  Definition auth_even_at (n: nat) := own even_name (●E n).
+  Definition auth_odd_at (n: nat) := own odd_name (●E n).
 
   Lemma they_agree γ (N M: nat):
     own γ (◯E N) -∗ own γ (●E M) -∗ ⌜ M = N ⌝.
@@ -112,11 +110,11 @@ Section proof.
     iDestruct (own_valid with "H") as "%Hval".
     iPureIntro. by apply excl_auth_agree_L.
   Qed.
-  Lemma yes_agree N M:
-    yes_at N -∗ auth_yes_at M -∗ ⌜ M = N ⌝.
+  Lemma even_agree N M:
+    even_at N -∗ auth_even_at M -∗ ⌜ M = N ⌝.
   Proof. apply they_agree. Qed.
-  Lemma no_agree N M:
-    no_at N -∗ auth_no_at M -∗ ⌜ M = N ⌝.
+  Lemma odd_agree N M:
+    odd_at N -∗ auth_odd_at M -∗ ⌜ M = N ⌝.
   Proof. apply they_agree. Qed.
 
   Lemma they_update γ (N M P: nat):
@@ -124,44 +122,38 @@ Section proof.
   Proof.
     rewrite -!own_op. iApply own_update. apply excl_auth_update.
   Qed.
-  Lemma yes_update P N M:
-     auth_yes_at M ∗ yes_at N ==∗ auth_yes_at P ∗ yes_at P.
+  Lemma even_update P N M:
+     auth_even_at M ∗ even_at N ==∗ auth_even_at P ∗ even_at P.
   Proof. apply they_update. Qed.
-  Lemma no_update P N M:
-     auth_no_at M ∗ no_at N ==∗ auth_no_at P ∗ no_at P.
+  Lemma odd_update P N M:
+     auth_odd_at M ∗ odd_at N ==∗ auth_odd_at P ∗ odd_at P.
   Proof. apply they_update. Qed.
 
-  Lemma they_finished_update γ (N M P: bool):
-    own γ (●E N) ∗ own γ (◯E M) ==∗ own γ (●E P) ∗ own γ (◯E P).
-  Proof.
-    rewrite -!own_op. iApply own_update. apply excl_auth_update.
-  Qed.
-
-  Definition yesno_inv_inner n :=
+  Definition evenodd_inv_inner n :=
     (∃ N,
           frag_free_roles_are ∅ ∗
           frag_model_is N ∗ n ↦ #N ∗
           (if (Nat.even N)
-           then auth_yes_at N ∗ auth_no_at (N+1)
-           else auth_yes_at (N+1) ∗ auth_no_at N))%I.
-  Definition yesno_inv n := inv Ns (yesno_inv_inner n).
+           then auth_even_at N ∗ auth_odd_at (N+1)
+           else auth_even_at (N+1) ∗ auth_odd_at N))%I.
+  Definition evenodd_inv n := inv Ns (evenodd_inv_inner n).
 
-  Lemma yes_go_spec tid n (N: nat) f (Hf: f > 40):
-    {{{ yesno_inv n ∗ has_fuel tid Y f ∗ yes_at N }}}
+  Lemma even_go_spec tid n (N: nat) f (Hf: f > 40):
+    {{{ evenodd_inv n ∗ has_fuel tid ρEven f ∗ even_at N }}}
       incr_loop #n #N @ tid
     {{{ RET #(); tid ↦M ∅ }}}.
   Proof.
     iLöb as "Hg" forall (N f Hf).
-    iIntros (Φ) "(#Hinv & Hf & Hyes) Hk".
+    iIntros (Φ) "(#Hinv & Hf & Heven) Hk".
     wp_lam.
     wp_pures.
     wp_bind (CmpXchg _ _ _).
     iApply wp_atomic.
     iInv Ns as (M) "(>HFR & >Hmod & >Hn & Hauths)" "Hclose".
     destruct (Nat.even M) eqn:Heqn; iDestruct "Hauths" as "[>Hay >Han]".
-    - iDestruct (yes_agree with "Hyes Hay") as "%Heq".
+    - iDestruct (even_agree with "Heven Hay") as "%Heq".
       rewrite -has_fuel_fuels.
-      iApply (wp_cmpxchg_suc_step_singlerole _ tid (Y: fmrole the_fair_model) _ 55%nat _
+      iApply (wp_cmpxchg_suc_step_singlerole _ tid (ρEven: fmrole the_fair_model) _ 55%nat _
                                              M (M + 1)
              with "[$]"); eauto.
       { by do 3 f_equiv. }
@@ -169,7 +161,7 @@ Section proof.
       { rewrite Nat.add_1_r. econstructor. eauto. }
       iModIntro.
       iIntros "!> (Hb & Hmod & HFR & Hf)".
-      iMod (yes_update (M + 2) with "[$]") as "[Hay Hyes]".
+      iMod (even_update (M + 2) with "[$]") as "[Hay Heven]".
       iMod ("Hclose" with "[Hmod Hay Han Hb HFR]").
       { iNext. iExists _. iFrame. rewrite Nat2Z.inj_add.
         subst. iFrame.
@@ -183,13 +175,13 @@ Section proof.
       rewrite has_fuel_fuels.
       wp_pures.
       replace (Z.of_nat N + 2)%Z with (Z.of_nat (N + 2)) by lia.
-      iApply ("Hg" with "[] [Hyes Hf] [$]"); last first.
+      iApply ("Hg" with "[] [Heven Hf] [$]"); last first.
       { iFrame "∗#". rewrite has_fuel_fuels.
         subst. iFrame. }
       iPureIntro; lia.
-    - iDestruct (yes_agree with "Hyes Hay") as "%Heq". rewrite -> Heq in *.
+    - iDestruct (even_agree with "Heven Hay") as "%Heq". rewrite -> Heq in *.
       rewrite -has_fuel_fuels.
-      iApply (wp_cmpxchg_fail_step_singlerole _ tid (Y: fmrole the_fair_model) _ 50%nat _
+      iApply (wp_cmpxchg_fail_step_singlerole _ tid (ρEven: fmrole the_fair_model) _ 50%nat _
                                              M M
              with "[$]"); eauto.
       { intros Hne. simplify_eq. lia. }
@@ -205,27 +197,27 @@ Section proof.
       iModIntro.
       wp_pures.
       rewrite -has_fuel_fuels.
-      iApply ("Hg" with "[] [Hyes Hf] [$]"); last first.
+      iApply ("Hg" with "[] [Heven Hf] [$]"); last first.
       { iFrame "∗#". }
       iPureIntro; lia.
   Qed.
 
-  Lemma no_go_spec tid n (N: nat) f (Hf: f > 40):
-    {{{ yesno_inv n ∗ has_fuel tid No f ∗ no_at N }}}
+  Lemma odd_go_spec tid n (N: nat) f (Hf: f > 40):
+    {{{ evenodd_inv n ∗ has_fuel tid ρOdd f ∗ odd_at N }}}
       incr_loop #n #N @ tid
     {{{ RET #(); tid ↦M ∅ }}}.
   Proof.
     iLöb as "Hg" forall (N f Hf).
-    iIntros (Φ) "(#Hinv & Hf & Hno) Hk".
+    iIntros (Φ) "(#Hinv & Hf & Hodd) Hk".
     wp_lam.
     wp_pures.
     wp_bind (CmpXchg _ _ _).
     iApply wp_atomic.
     iInv Ns as (M) "(>HFR & >Hmod & >Hn & Hauths)" "Hclose".
     destruct (Nat.even M) eqn:Heqn; iDestruct "Hauths" as "[>Hay >Han]"; last first.
-    - iDestruct (no_agree with "Hno Han") as "%Heq".
+    - iDestruct (odd_agree with "Hodd Han") as "%Heq".
       rewrite -has_fuel_fuels.
-      iApply (wp_cmpxchg_suc_step_singlerole _ tid (No: fmrole the_fair_model) _ 55%nat _
+      iApply (wp_cmpxchg_suc_step_singlerole _ tid (ρOdd: fmrole the_fair_model) _ 55%nat _
                                              M (S M)
                with "[$]"); eauto.
       { by do 3 f_equiv. }
@@ -233,7 +225,7 @@ Section proof.
       { econstructor. rewrite -Nat.negb_even. rewrite Heqn. done. }
       iModIntro.
       iIntros "!> (Hb & Hmod & HFR & Hf)".
-      iMod (no_update (M + 2) with "[$]") as "[Han Hno]".
+      iMod (odd_update (M + 2) with "[$]") as "[Han Hodd]".
       iMod ("Hclose" with "[Hmod Hay Han Hb HFR]").
       { iNext. iExists _. iFrame. subst.
         rewrite Nat.add_1_r.
@@ -251,12 +243,12 @@ Section proof.
       wp_pures.
       rewrite -has_fuel_fuels.
       replace (Z.of_nat N + 2)%Z with (Z.of_nat (N + 2)) by lia.
-      iApply ("Hg" with "[] [Hno Hf] [$]"); last first.
+      iApply ("Hg" with "[] [Hodd Hf] [$]"); last first.
       { iFrame "∗#". simplify_eq. done. }
       iPureIntro; lia.
-    - iDestruct (no_agree with "Hno Han") as "%Heq". rewrite -> Heq in *.
+    - iDestruct (odd_agree with "Hodd Han") as "%Heq". rewrite -> Heq in *.
       rewrite -has_fuel_fuels. simplify_eq.
-      iApply (wp_cmpxchg_fail_step_singlerole _ tid (No: fmrole the_fair_model) _ 50%nat _
+      iApply (wp_cmpxchg_fail_step_singlerole _ tid (ρOdd: fmrole the_fair_model) _ 50%nat _
                                              M M
              with "[$]"); eauto.
       { intros Hneq. simplify_eq. lia. }
@@ -271,41 +263,41 @@ Section proof.
       iModIntro.
       wp_pures.
       rewrite -has_fuel_fuels.
-      iApply ("Hg" with "[] [Hno Hf] [$]"); last first.
+      iApply ("Hg" with "[] [Hodd Hf] [$]"); last first.
       { iFrame "∗#". }
       iPureIntro; lia.
   Qed.
 
-  Definition role_frag (yn : YN) : nat → iProp Σ :=
-    match yn with
-    | Y => yes_at
-    | No => no_at
+  Definition role_frag (eo : EO) : nat → iProp Σ :=
+    match eo with
+    | ρEven => even_at
+    | ρOdd => odd_at
     end.
 
-  Lemma incr_loop_spec tid n (N : nat) f (Hf: f > 40) (yn : YN) :
-    {{{ yesno_inv n ∗ has_fuel tid yn f ∗ (role_frag yn) N }}}
+  Lemma incr_loop_spec tid n (N : nat) f (Hf: f > 40) (eo : EO) :
+    {{{ evenodd_inv n ∗ has_fuel tid eo f ∗ (role_frag eo) N }}}
       incr_loop #n #N @ tid
     {{{ RET #(); tid ↦M ∅ }}}.
   Proof.
-    iIntros (Φ) "(#Hinv & Hf & Hyn) Hk".
-    destruct yn.
-    - iApply (yes_go_spec with "[$Hf $Hyn]"); [lia|done|done].
-    - iApply (no_go_spec with "[$Hf $Hyn]"); [lia|done|done].
+    iIntros (Φ) "(#Hinv & Hf & Heo) Hk".
+    destruct eo.
+    - iApply (even_go_spec with "[$Hf $Heo]"); [lia|done|done].
+    - iApply (odd_go_spec with "[$Hf $Heo]"); [lia|done|done].
   Qed.
 
 End proof.
 
 Section proof_start.
-  Context `{!heapGS Σ the_model, !yesnoG Σ}.
-  Let Ns := nroot .@ "yes_no".
+  Context `{!heapGS Σ the_model, !evenoddG Σ}.
+  Let Ns := nroot .@ "even_odd".
 
   Lemma start_spec tid n N1 N2 f (Hf: f > 60) :
-    {{{ yesno_inv n ∗ has_fuels tid {[ Y := f; No := f ]} ∗
-        yes_at N1 ∗ no_at N2 }}}
+    {{{ evenodd_inv n ∗ has_fuels tid {[ ρEven := f; ρOdd := f ]} ∗
+        even_at N1 ∗ odd_at N2 }}}
       start #n @ tid
     {{{ RET #(); tid ↦M ∅ }}}.
   Proof using All.
-    iIntros (Φ) "(#Hinv & Hf & Hyes_at & Hno_at) HΦ". unfold start.
+    iIntros (Φ) "(#Hinv & Hf & Heven_at & Hodd_at) HΦ". unfold start.
     wp_pures.
     wp_bind (Load _).
     iApply wp_atomic.
@@ -314,15 +306,15 @@ Section proof_start.
     wp_load.
     iIntros "!>".
     destruct (Nat.even M) eqn:Heven.
-    - iDestruct "Hauths" as "[Hyes Hno]".
-      iDestruct (yes_agree with "Hyes_at Hyes") as %<-.
-      iDestruct (no_agree with "Hno_at Hno") as %<-.
-      iMod ("Hclose" with "[-Hf Hyes_at Hno_at HΦ]") as "_".
+    - iDestruct "Hauths" as "[Heven Hodd]".
+      iDestruct (even_agree with "Heven_at Heven") as %<-.
+      iDestruct (odd_agree with "Hodd_at Hodd") as %<-.
+      iMod ("Hclose" with "[-Hf Heven_at Hodd_at HΦ]") as "_".
       { iIntros "!>". iExists _. iFrame. rewrite Heven. iFrame. }
       iIntros "!>". wp_pures. wp_bind (Fork _).
       rewrite has_fuels_gt_1; last solve_fuel_positive.
-      iApply (wp_fork_nostep _ tid _ _ _ {[ No ]} {[ Y ]} {[Y := _; No := _]}
-               with "[Hyes_at] [- Hf] [Hf]");
+      iApply (wp_fork_nostep _ tid _ _ _ {[ ρOdd ]} {[ ρEven ]} {[ρEven := _; ρOdd := _]}
+               with "[Heven_at] [- Hf] [Hf]");
         [ set_solver | by apply insert_non_empty | | | |
           rewrite !fmap_insert fmap_empty // ]; [set_solver | |].
       { iIntros (tid') "!> Hf".
@@ -330,7 +322,7 @@ Section proof_start.
         rewrite map_filter_insert_not; last set_solver.
         rewrite map_filter_empty insert_empty.
         rewrite -has_fuel_fuels.
-        iApply (incr_loop_spec with "[Hyes_at $Hf]"); [lia|iFrame "#∗"|].
+        iApply (incr_loop_spec with "[Heven_at $Hf]"); [lia|iFrame "#∗"|].
         by iIntros "!>?". }
       iIntros "!> Hf".
       iIntros "!>".
@@ -339,7 +331,7 @@ Section proof_start.
       rewrite map_filter_empty insert_empty.
       wp_pures.
       rewrite has_fuels_gt_1; last solve_fuel_positive.
-      iApply (wp_fork_nostep _ tid _ _ _ ∅ {[ No ]} {[No := _]} with "[Hno_at] [HΦ] [Hf]");
+      iApply (wp_fork_nostep _ tid _ _ _ ∅ {[ ρOdd ]} {[ρOdd := _]} with "[Hodd_at] [HΦ] [Hf]");
         [ set_solver | by apply insert_non_empty | | | |
           rewrite !fmap_insert fmap_empty // ]; [set_solver| |].
       + iIntros (tid') "!> Hf".
@@ -349,7 +341,7 @@ Section proof_start.
         wp_pures.
         rewrite -has_fuel_fuels.
         replace (Z.of_nat M + 1)%Z with (Z.of_nat (M + 1)) by lia.
-        iApply (incr_loop_spec with "[Hno_at $Hf]"); [lia|iFrame "#∗"|].
+        iApply (incr_loop_spec with "[Hodd_at $Hf]"); [lia|iFrame "#∗"|].
         by iIntros "!>?".
     + iIntros "!> Hf".
         rewrite map_filter_insert_not; last set_solver.
@@ -357,16 +349,16 @@ Section proof_start.
         iApply "HΦ". iModIntro.
         iDestruct "Hf" as "[Hf _]".
         by rewrite dom_empty_L.
-    - iDestruct "Hauths" as "[Hyes Hno]".
-      iDestruct (yes_agree with "Hyes_at Hyes") as %<-.
-      iDestruct (no_agree with "Hno_at Hno") as %<-.
-      iMod ("Hclose" with "[-Hf Hyes_at Hno_at HΦ]") as "_".
+    - iDestruct "Hauths" as "[Heven Hodd]".
+      iDestruct (even_agree with "Heven_at Heven") as %<-.
+      iDestruct (odd_agree with "Hodd_at Hodd") as %<-.
+      iMod ("Hclose" with "[-Hf Heven_at Hodd_at HΦ]") as "_".
       { iIntros "!>". iExists _. iFrame. rewrite Heven. iFrame. }
       iIntros "!>". wp_pures. wp_bind (Fork _).
       rewrite has_fuels_gt_1; last solve_fuel_positive.
       rewrite insert_commute; [|done].
-      iApply (wp_fork_nostep _ tid _ _ _ {[ Y ]} {[ No ]} {[No := _; Y := _]}
-               with "[Hno_at] [- Hf] [Hf]");
+      iApply (wp_fork_nostep _ tid _ _ _ {[ ρEven ]} {[ ρOdd ]} {[ρOdd := _; ρEven := _]}
+               with "[Hodd_at] [- Hf] [Hf]");
         [ set_solver | by apply insert_non_empty | | | |
           rewrite !fmap_insert fmap_empty // ]; [set_solver | |].
       { iIntros (tid') "!> Hf".
@@ -374,7 +366,7 @@ Section proof_start.
         rewrite map_filter_insert_not; last set_solver.
         rewrite map_filter_empty insert_empty.
         rewrite -has_fuel_fuels.
-        iApply (incr_loop_spec with "[Hno_at $Hf]"); [lia|iFrame "#∗"|].
+        iApply (incr_loop_spec with "[Hodd_at $Hf]"); [lia|iFrame "#∗"|].
         by iIntros "!>?". }
       iIntros "!> Hf".
       iIntros "!>".
@@ -383,7 +375,7 @@ Section proof_start.
       rewrite map_filter_empty insert_empty.
       wp_pures.
       rewrite has_fuels_gt_1; last solve_fuel_positive.
-      iApply (wp_fork_nostep _ tid _ _ _ ∅ {[ Y ]} {[Y := _]} with "[Hyes_at] [HΦ] [Hf]");
+      iApply (wp_fork_nostep _ tid _ _ _ ∅ {[ ρEven ]} {[ρEven := _]} with "[Heven_at] [HΦ] [Hf]");
         [ set_solver | by apply insert_non_empty | | | |
           rewrite !fmap_insert fmap_empty // ]; [set_solver| |].
       + iIntros (tid') "!> Hf".
@@ -393,7 +385,7 @@ Section proof_start.
         wp_pures.
         rewrite -has_fuel_fuels.
         replace (Z.of_nat M + 1)%Z with (Z.of_nat (M + 1)) by lia.
-        iApply (incr_loop_spec with "[Hyes_at $Hf]"); [lia|iFrame "#∗"|].
+        iApply (incr_loop_spec with "[Heven_at $Hf]"); [lia|iFrame "#∗"|].
         by iIntros "!>?".
       + iIntros "!> Hf".
         rewrite map_filter_insert_not; last set_solver.
