fairness/examples/yesno_incr/yesno_incr_adequacy.v
@@ -29,17 +29,17 @@ Proof. intros Heven Hodd. by eapply even_odd_False. Qed.
 
 (** The model is finitely branching *)
 
-Definition steppable n : list (nat * option YN) :=
+Definition steppable n : list (nat * option EO) :=
   n' ← [S n; n];
-  ℓ ← [Some Y; Some No];
+  ℓ ← [Some ρEven; Some ρOdd];
   mret (n', ℓ).
 
 #[local] Instance proof_irrel_trans s x:
-  ProofIrrel ((let '(s', ℓ) := x in yntrans s ℓ s'): Prop).
+  ProofIrrel ((let '(s', ℓ) := x in eotrans s ℓ s'): Prop).
 Proof. apply make_proof_irrel. Qed.
 
 Lemma model_finitary s:
-  Finite { '(s', ℓ) | yntrans s ℓ s'}.
+  Finite { '(s', ℓ) | eotrans s ℓ s'}.
 Proof.
   assert (H: forall A (y x: A) xs, (y = x ∨ y ∈ xs) -> y ∈ x::xs) by set_solver.
   eapply (in_list_finite (steppable s)).
@@ -50,12 +50,12 @@ Qed.
 
 (** Proof that any fair execution of model visits all natural numbers *)
 
-Definition yesno_mtrace : Type := mtrace the_fair_model.
+Definition evenodd_mtrace : Type := mtrace the_fair_model.
 
-Definition yesno_mdl_progress (tr : yesno_mtrace) :=
+Definition evenodd_mdl_progress (tr : evenodd_mtrace) :=
   ∀ n, ∃ m, pred_at tr m (λ s _, s = n).
 
-Lemma yesno_mdl_always_live ρ n (mtr : yesno_mtrace) :
+Lemma evenodd_mdl_always_live ρ n (mtr : evenodd_mtrace) :
   infinite_trace mtr →
   pred_at mtr n
           (λ (δ : the_fair_model) (_ : option (option (fmrole the_fair_model))),
@@ -66,28 +66,28 @@ Proof.
   destruct mtr'; destruct ρ; set_solver.
 Qed.
 
-Lemma yesno_mdl_always_eventually_scheduled ρ (mtr : yesno_mtrace) :
+Lemma evenodd_mdl_always_eventually_scheduled ρ (mtr : evenodd_mtrace) :
   infinite_trace mtr → fair_model_trace ρ mtr →
   ∀ n, ∃ m, pred_at mtr (n+m) (λ _ ℓ, ℓ = Some (Some ρ)).
 Proof.
   intros Hinf Hfair n.
-  apply (yesno_mdl_always_live ρ n mtr) in Hinf.
+  apply (evenodd_mdl_always_live ρ n mtr) in Hinf.
   specialize (Hfair n Hinf) as [m [Hfair | Hfair]].
   - rewrite /pred_at in Hfair. destruct (after (n + m) mtr); [|done].
     rewrite /role_enabled_model in Hfair. destruct t; destruct ρ; set_solver.
   - by exists m.
 Qed.
 
-Lemma yesno_mdl_noprogress_Y i n (mtr : yesno_mtrace) :
+Lemma evenodd_mdl_noprogress_Even i n (mtr : evenodd_mtrace) :
   infinite_trace mtr → mtrace_valid mtr → (trfirst mtr) = i → Nat.even i →
-  (∀ m, m < n → pred_at mtr m (λ _ l, l ≠ Some (Some Y))) →
+  (∀ m, m < n → pred_at mtr m (λ _ l, l ≠ Some (Some ρEven))) →
   pred_at mtr n (λ s _, s = i).
 Proof.
   intros Hinf Hvalid Hfirst Heven Hne.
   induction n as [|n IHn].
   { rewrite /pred_at. destruct mtr; done. }
   simpl in *.
-  assert (∀ m : nat, m < n → pred_at mtr m (λ _ l, l ≠ Some (Some Y))) as Hne'.
+  assert (∀ m : nat, m < n → pred_at mtr m (λ _ l, l ≠ Some (Some ρEven))) as Hne'.
   { intros. apply Hne. lia. }
   specialize (IHn Hne'). rewrite /pred_at in IHn.
   destruct (after n mtr) as [mtr'|] eqn:Hafter; rewrite Hafter in IHn; [|done].
@@ -96,7 +96,7 @@ Proof.
   rewrite after_sum' in Hinf. rewrite Hafter in Hinf.
   destruct mtr'; [by apply is_Some_None in Hinf|].
   eapply mtrace_valid_after in Hvalid; [|done].
-  assert (ℓ ≠ Some Y) as Hneq.
+  assert (ℓ ≠ Some ρEven) as Hneq.
   { assert (n < S n) by lia. specialize (Hne n H). rewrite /pred_at in Hne.
     rewrite Hafter in Hne. intros ->. apply Hne. done. }
   pinversion Hvalid. simplify_eq. inversion H1; simplify_eq.
@@ -104,16 +104,16 @@ Proof.
   - by destruct mtr'.
 Qed.
 
-Lemma yesno_mdl_noprogress_No i n (mtr : yesno_mtrace) :
+Lemma evenodd_mdl_noprogress_Odd i n (mtr : evenodd_mtrace) :
   infinite_trace mtr → mtrace_valid mtr → (trfirst mtr) = i → Nat.odd i →
-  (∀ m, m < n → pred_at mtr m (λ _ l, l ≠ Some (Some No))) →
+  (∀ m, m < n → pred_at mtr m (λ _ l, l ≠ Some (Some ρOdd))) →
   pred_at mtr n (λ s _, s = i).
 Proof.
   intros Hinf Hvalid Hfirst Hodd Hne.
   induction n as [|n IHn].
   { rewrite /pred_at. destruct mtr; done. }
   simpl in *.
-  assert (∀ m : nat, m < n → pred_at mtr m (λ _ l, l ≠ Some (Some No))) as Hne'.
+  assert (∀ m : nat, m < n → pred_at mtr m (λ _ l, l ≠ Some (Some ρOdd))) as Hne'.
   { intros. apply Hne. lia. }
   specialize (IHn Hne'). rewrite /pred_at in IHn.
   destruct (after n mtr) as [mtr'|] eqn:Hafter; rewrite Hafter in IHn; [|done].
@@ -122,7 +122,7 @@ Proof.
   rewrite after_sum' in Hinf. rewrite Hafter in Hinf.
   destruct mtr'; [by apply is_Some_None in Hinf|].
   eapply mtrace_valid_after in Hvalid; [|done].
-  assert (ℓ ≠ Some No) as Hneq.
+  assert (ℓ ≠ Some ρOdd) as Hneq.
   { assert (n < S n) by lia. specialize (Hne n H). rewrite /pred_at in Hne.
     rewrite Hafter in Hne. intros ->. apply Hne. done. }
   pinversion Hvalid. simplify_eq. inversion H1; simplify_eq.
@@ -130,14 +130,14 @@ Proof.
   - by destruct mtr'.
 Qed.
 
-Theorem yesno_mdl_progresses_Y i (mtr : yesno_mtrace) :
+Theorem evenodd_mdl_progresses_Even i (mtr : evenodd_mtrace) :
   infinite_trace mtr → mtrace_valid mtr → (∀ ρ, fair_model_trace ρ mtr) →
   (trfirst mtr) = i → Nat.even i →
   ∃ m, pred_at mtr m (λ s _, s = S i).
 Proof.
   intros Hinf Hvalid Hfair Hfirst Heven.
-  specialize (Hfair Y).
-  pose proof (yesno_mdl_always_eventually_scheduled Y mtr Hinf Hfair 0) as Hsched.
+  specialize (Hfair ρEven).
+  pose proof (evenodd_mdl_always_eventually_scheduled ρEven mtr Hinf Hfair 0) as Hsched.
   simpl in *. apply trace_eventually_until in Hsched as [m [Hsched Hschedne]].
   rewrite /pred_at in Hsched.
   destruct (after m mtr) as [mtr'|] eqn:Hafter; last first.
@@ -146,7 +146,7 @@ Proof.
   destruct mtr'; [done|].
   simplify_eq.
   assert (s = trfirst mtr) as ->.
-  { eapply yesno_mdl_noprogress_Y in Hschedne; [|done..].
+  { eapply evenodd_mdl_noprogress_Even in Hschedne; [|done..].
     rewrite /pred_at in Hschedne. rewrite Hafter in Hschedne. done. }
   eapply mtrace_valid_after in Hvalid; [|done].
   pinversion Hvalid; simplify_eq. inversion H1; simplify_eq.
@@ -156,14 +156,14 @@ Proof.
   - by apply even_not_odd in Heven.
 Qed.
 
-Theorem yesno_mdl_progresses_No i (mtr : yesno_mtrace) :
+Theorem evenodd_mdl_progresses_Odd i (mtr : evenodd_mtrace) :
   infinite_trace mtr → mtrace_valid mtr → (∀ ρ, fair_model_trace ρ mtr) →
   (trfirst mtr) = i → Nat.odd i →
   ∃ m, pred_at mtr m (λ s _, s = S i).
 Proof.
   intros Hinf Hvalid Hfair Hfirst Hodd.
-  specialize (Hfair No).
-  pose proof (yesno_mdl_always_eventually_scheduled No mtr Hinf Hfair 0) as Hsched.
+  specialize (Hfair ρOdd).
+  pose proof (evenodd_mdl_always_eventually_scheduled ρOdd mtr Hinf Hfair 0) as Hsched.
   simpl in *. apply trace_eventually_until in Hsched as [m [Hsched Hschedne]].
   rewrite /pred_at in Hsched.
   destruct (after m mtr) as [mtr'|] eqn:Hafter; last first.
@@ -172,7 +172,7 @@ Proof.
   destruct mtr'; [done|].
   simplify_eq.
   assert (s = trfirst mtr) as ->.
-  { eapply yesno_mdl_noprogress_No in Hschedne; [|done..].
+  { eapply evenodd_mdl_noprogress_Odd in Hschedne; [|done..].
     rewrite /pred_at in Hschedne. rewrite Hafter in Hschedne. done. }
   eapply mtrace_valid_after in Hvalid; [|done].
   pinversion Hvalid; simplify_eq. inversion H1; simplify_eq.
@@ -182,10 +182,10 @@ Proof.
   - by apply odd_not_even in Hodd.
 Qed.
 
-Theorem yesno_mdl_progresses (mtr : yesno_mtrace) :
+Theorem evenodd_mdl_progresses (mtr : evenodd_mtrace) :
   infinite_trace mtr → mtrace_valid mtr → (∀ ρ, fair_model_trace ρ mtr) →
   (trfirst mtr) = 0 →
-  yesno_mdl_progress mtr.
+  evenodd_mdl_progress mtr.
 Proof.
   intros Hinf Hvalid Hfair Hfirst i.
   induction i as [|i IHi].
@@ -201,7 +201,7 @@ Proof.
     { intros. by eapply fair_model_trace_after. }
     assert (trfirst mtr' = i) as Hfirst'.
     { rewrite /trfirst. destruct mtr'; done. }
-    pose proof (yesno_mdl_progresses_Y i mtr' Hinf Hvalid Hfair' Hfirst')
+    pose proof (evenodd_mdl_progresses_Even i mtr' Hinf Hvalid Hfair' Hfirst')
       as [m Hpred']; [by eauto|].
     exists (n + m).
     rewrite pred_at_sum. rewrite Hafter. done.
@@ -209,7 +209,7 @@ Proof.
     { intros. by eapply fair_model_trace_after. }
     assert (trfirst mtr' = i) as Hfirst'.
     { rewrite /trfirst. destruct mtr'; done. }
-    pose proof (yesno_mdl_progresses_No i mtr' Hinf Hvalid Hfair' Hfirst')
+    pose proof (evenodd_mdl_progresses_Odd i mtr' Hinf Hvalid Hfair' Hfirst')
       as [m Hpred']; [by rewrite -Nat.negb_even Heqn|].
     exists (n + m).
     rewrite pred_at_sum. rewrite Hafter. done.
@@ -217,14 +217,14 @@ Qed.
 
 (** Proof that fair progress is preserved through auxiliary trace *)
 
-Definition yesno_aux_progress (auxtr : auxtrace the_model) :=
+Definition evenodd_aux_progress (auxtr : auxtrace the_model) :=
   ∀ n, ∃ m, pred_at auxtr m (λ s l, (λ s' _, s' = n) (ls_under s) (l ≫= Ul)).
 
-Lemma yesno_mtr_aux_progress_preserved
+Lemma evenodd_mtr_aux_progress_preserved
       (mtr : mtrace the_fair_model)
       (auxtr : auxtrace the_model) :
   upto_stutter ls_under Ul auxtr mtr →
-  yesno_mdl_progress mtr → yesno_aux_progress auxtr.
+  evenodd_mdl_progress mtr → evenodd_aux_progress auxtr.
 Proof.
   intros Hstutter Hmtr n. specialize (Hmtr n).
   by apply (trace_eventually_stutter_preserves
@@ -234,27 +234,27 @@ Qed.
 (** Proof that progress is preserved between auxilary and execution trace,
  for a specific ξ *)
 
-Definition yesno_ex_progress (l:loc) (extr : heap_lang_extrace) :=
+Definition evenodd_ex_progress (l:loc) (extr : heap_lang_extrace) :=
   ∀ (n:nat), ∃ m, pred_at extr m (λ s _, heap s.2 !! l = Some #n).
 
-Definition ξ_yesno_model_match (l : loc) (c : cfg heap_lang) (δ : the_fair_model) :=
+Definition ξ_evenodd_model_match (l : loc) (c : cfg heap_lang) (δ : the_fair_model) :=
   ∃ (N:nat), heap c.2 !! l = Some #N ∧ δ = N.
 
-Definition ξ_yesno_no_val_steps (c : cfg heap_lang) (δ : the_fair_model) :=
+Definition ξ_evenodd_no_val_steps (c : cfg heap_lang) (δ : the_fair_model) :=
   (Forall (λ e, is_Some $ to_val e) c.1 → False) ∧
   Forall (λ e, not_stuck e c.2) c.1.
 
-Definition ξ_yesno (l : loc) (c : cfg heap_lang) (δ : the_fair_model) :=
-  ξ_yesno_no_val_steps c δ ∧ ξ_yesno_model_match l c δ.
+Definition ξ_evenodd (l : loc) (c : cfg heap_lang) (δ : the_fair_model) :=
+  ξ_evenodd_no_val_steps c δ ∧ ξ_evenodd_model_match l c δ.
 
-Definition ξ_yesno_trace (l : loc) (extr : execution_trace heap_lang)
-           (auxtr : finite_trace the_fair_model (option YN)) :=
-  ξ_yesno l (trace_last extr) (trace_last auxtr).
+Definition ξ_evenodd_trace (l : loc) (extr : execution_trace heap_lang)
+           (auxtr : finite_trace the_fair_model (option EO)) :=
+  ξ_evenodd l (trace_last extr) (trace_last auxtr).
 
-Lemma yesno_aux_ex_progress_preserved l (extr : heap_lang_extrace) (auxtr : auxtrace the_model) :
-  traces_match labels_match (λ c δ, live_tids c δ ∧ ξ_yesno l c δ) locale_step
+Lemma evenodd_aux_ex_progress_preserved l (extr : heap_lang_extrace) (auxtr : auxtrace the_model) :
+  traces_match labels_match (λ c δ, live_tids c δ ∧ ξ_evenodd l c δ) locale_step
   (lm_ls_trans the_model) extr auxtr →
-  yesno_aux_progress auxtr → yesno_ex_progress l extr.
+  evenodd_aux_progress auxtr → evenodd_ex_progress l extr.
 Proof.
   intros Hξ Hauxtr n. specialize (Hauxtr n).
   rewrite /pred_at in Hauxtr. destruct Hauxtr as [m Hauxtr].
@@ -271,51 +271,51 @@ Proof. intros x y. apply make_decision. Qed.
 Instance the_model_mlabel_countable : EqDecision (mlabel the_model).
 Proof. solve_decision. Qed.
 
-(** Proof that program refines model up to ξ_yesno *)
+(** Proof that program refines model up to ξ_evenodd *)
 
-Lemma yesno_incr_sim l :
+Lemma evenodd_incr_sim l :
   continued_simulation
-    (sim_rel_with_user the_model (ξ_yesno_trace l))
+    (sim_rel_with_user the_model (ξ_evenodd_trace l))
     (trace_singleton ([start #l],
                         {| heap := {[l:=#0]};
                            used_proph_id := ∅ |}))
     (trace_singleton (initial_ls (LM := the_model) 0 0)).
 Proof.
-  assert (yesnoPreG yesnoΣ) as HPreG'.
+  assert (evenoddPreG evenoddΣ) as HPreG'.
   { apply _. }
-  assert (heapGpreS yesnoΣ the_model) as HPreG.
+  assert (heapGpreS evenoddΣ the_model) as HPreG.
   { apply _. }
   eapply (strong_simulation_adequacy
-            yesnoΣ _ NotStuck _ _ _ ∅); [|set_solver|].
+            evenoddΣ _ NotStuck _ _ _ ∅); [|set_solver|].
   { eapply rel_finitary_sim_rel_with_user_sim_rel.
     eapply valid_state_evolution_finitary_fairness_simple.
     intros ?. simpl. apply (model_finitary s1). }
   iIntros (?) "!> Hσ Hs Hr Hf".
-  iMod (own_alloc (●E 0  ⋅ ◯E 0))%nat as (γ_yes_at) "[Hyes_at_auth Hyes_at]".
+  iMod (own_alloc (●E 0  ⋅ ◯E 0))%nat as (γ_even_at) "[Heven_at_auth Heven_at]".
   { apply auth_both_valid_2; eauto. by compute. }
-  iMod (own_alloc (●E 1  ⋅ ◯E 1))%nat as (γ_no_at) "[Hno_at_auth Hno_at]".
+  iMod (own_alloc (●E 1  ⋅ ◯E 1))%nat as (γ_odd_at) "[Hodd_at_auth Hodd_at]".
   { apply auth_both_valid_2; eauto. by compute. }
   pose (the_names := {|
-   yes_name := γ_yes_at;
-   no_name := γ_no_at;
+   even_name := γ_even_at;
+   odd_name := γ_odd_at;
   |}).
-  iMod (inv_alloc (nroot .@ "yes_no") _ (yesno_inv_inner l) with "[Hσ Hs Hr Hyes_at_auth Hno_at_auth]") as "#Hinv".
-  { iNext. unfold yesno_inv_inner. iExists 0.
+  iMod (inv_alloc (nroot .@ "even_odd") _ (evenodd_inv_inner l) with "[Hσ Hs Hr Heven_at_auth Hodd_at_auth]") as "#Hinv".
+  { iNext. unfold evenodd_inv_inner. iExists 0.
     replace (∅ ∖ live_roles the_fair_model 0) with
       (∅:gset (fmrole the_fair_model)) by set_solver.
-    rewrite /yn_live_roles big_sepM_singleton. by iFrame. }
+    rewrite /eo_live_roles big_sepM_singleton. by iFrame. }
   iModIntro.
   iSplitL.
-  { simpl. rewrite /yn_live_roles.
-    replace (gset_to_gmap 61 {[No; Y]}) with
-      ({[Y := 61; No := 61]} : gmap _ _); last first.
+  { simpl. rewrite /eo_live_roles.
+    replace (gset_to_gmap 61 {[ρOdd; ρEven]}) with
+      ({[ρEven := 61; ρOdd := 61]} : gmap _ _); last first.
     { rewrite /gset_to_gmap. simpl.
       rewrite !map_fmap_union. rewrite !map_fmap_singleton.
       rewrite map_union_comm; last first.
       { rewrite map_disjoint_singleton_l.
         by rewrite lookup_insert_ne. }
       by rewrite -!insert_union_l left_id. }
-    iApply (start_spec with "[$Hf $Hyes_at $Hno_at $Hinv]"); [lia|].
+    iApply (start_spec with "[$Hf $Heven_at $Hodd_at $Hinv]"); [lia|].
     by iIntros "!>?". }
   iIntros (extr auxtr c) "_ _ _ %Hends _ %Hnstuck [_ [Hσ Hδ]] Hposts".
   iInv "Hinv" as (M) "(>HFR & >Hmod & >Hn & _)" "Hclose".
@@ -382,7 +382,7 @@ Proof.
       - eapply (ls_mapping_dom (M:=the_fair_model)).
       - erewrite Hmapping. done. }
     rewrite /live_roles in Hlive. simpl in *.
-    rewrite /yn_live_roles in Hlive. set_solver.
+    rewrite /eo_live_roles in Hlive. set_solver.
   - iPureIntro.
     apply Forall_forall.
     intros e He. by apply Hnstuck.
@@ -413,20 +413,20 @@ Proof.
 Qed.
 
 (** Proof that execution trace actually progresses *)
-Theorem yesno_ex_progresses (l:loc) (extr : heap_lang_extrace) :
+Theorem evenodd_ex_progresses (l:loc) (extr : heap_lang_extrace) :
   extrace_maximal extr →
   (∀ tid, fair_ex tid extr) →
   trfirst extr = ([start #l],
                         {| heap := {[l:=#0]};
                            used_proph_id := ∅ |}) →
-  yesno_ex_progress l extr.
+  evenodd_ex_progress l extr.
 Proof.
   intros Hmaximal Hfair Hfirst.
   pose proof Hmaximal as Hvalid%extrace_maximal_valid.
-  pose proof (yesno_incr_sim l) as Hsim.
+  pose proof (evenodd_incr_sim l) as Hsim.
   assert (∃ iatr,
              valid_inf_system_trace
-               (continued_simulation (sim_rel_with_user the_model (ξ_yesno_trace l)))
+               (continued_simulation (sim_rel_with_user the_model (ξ_evenodd_trace l)))
                (trace_singleton (trfirst extr))
                (trace_singleton (initial_ls (LM:=the_model) 0 0))
                (from_trace extr)
@@ -437,12 +437,12 @@ Proof.
     - eapply from_trace_preserves_validity; eauto; first econstructor. }
   assert (∃ (auxtr : auxtrace the_model),
              traces_match labels_match
-               (live_tids /2\ (ξ_yesno l))
+               (live_tids /2\ (ξ_evenodd l))
                locale_step
                the_model.(lm_ls_trans) extr auxtr) as [auxtr Hmatch_strong].
   { exists (to_trace (initial_ls (LM := the_model) 0 0 ) iatr).
     eapply (valid_inf_system_trace_implies_traces_match_strong
-              (continued_simulation (sim_rel_with_user the_model (ξ_yesno_trace l)))); eauto.
+              (continued_simulation (sim_rel_with_user the_model (ξ_evenodd_trace l)))); eauto.
     - intros ? ? ?%continued_simulation_rel. by destruct H as [[_ H] _].
     - intros ? ? ?%continued_simulation_rel. by destruct H as [[H _] _].
     - intros extr' auxtr' ?%continued_simulation_rel.
@@ -506,8 +506,8 @@ Proof.
     assert (0 = ls_under (trfirst auxtr)) as Hσ' by lia.
     inversion Hupto; simplify_eq;
     by rewrite Hσ'. }
-  pose proof (yesno_mdl_progresses mtr Hinf'' Hvalid'' Hfair'' Hfirst'')
+  pose proof (evenodd_mdl_progresses mtr Hinf'' Hvalid'' Hfair'' Hfirst'')
     as Hprogress.
-  eapply (yesno_aux_ex_progress_preserved l _ auxtr); [done|].
-  by eapply yesno_mtr_aux_progress_preserved.
+  eapply (evenodd_aux_ex_progress_preserved l _ auxtr); [done|].
+  by eapply evenodd_mtr_aux_progress_preserved.
 Qed.
